Some tidying

typing/pure_typingScript.sml
@@ -5,9 +5,8 @@ open pure_cexpTheory pure_configTheory;
 
 val _ = new_theory "pure_typing";
 
-Definition data_reserved_cns_def:
-  data_reserved_cns = ""::"True"::"False"::reserved_cns
-End
+
+(******************** Types ********************)
 
 Datatype:
   prim_ty = Integer | String | Message | Bool
@@ -25,6 +24,160 @@ Datatype:
 End
 
 Overload Unit = ``Tuple []``;
+
+Type type_scheme[pp] = ``:num # type``;
+
+(*
+  A type definition is an arity and a collection of constructor definitions.
+  Each constructor definition is a name and a type scheme for its arguments
+  (closed wrt the type definition arity).
+
+  Like CakeML, use numbers to refer to types - known typedefs represented as
+    : typedef list
+  We could instead have:
+    : (string # typedef) list     or     : string |-> typedef     etc.
+  Unlike CakeML, we group constructors by their type (i.e. group siblings).
+
+  E.g. the type definitions for Maybe and List might look like:
+  [
+    (1, [ ("Nothing", []) ; ("Just", [Var 0]) ]);
+    (1, [ ("Nil", []) ; ("Cons", [Var 0; TypeCons 1 [Var 0]]) ])
+  ]
+
+  The exception definition is a list of constructors associated to (closed)
+  argument types.
+
+  Together, the exception definition and a collection of type definitions form
+  our typing namespace.
+*)
+Type typedef[pp] = ``:num # ((string # type list) list)``;
+Type typedefs[pp] = ``:typedef list``;
+Type exndef[pp] = ``:(string # type list) list``;
+
+
+(********** Substitutions and shifts **********)
+
+Definition subst_db_def:
+  subst_db skip ts (TypeVar v) = (
+    if skip ≤ v ∧ v < skip + LENGTH ts then
+      EL (v - skip) ts
+    else if skip ≤ v then
+      TypeVar (v - LENGTH ts)
+    else TypeVar v) ∧
+  subst_db skip ts (PrimTy p) = PrimTy p ∧
+  subst_db skip ts  Exception = Exception ∧
+  subst_db skip ts (TypeCons n tcs) = TypeCons n (MAP (subst_db skip ts) tcs) ∧
+  subst_db skip ts (Tuple tcs) = Tuple  (MAP (subst_db skip ts) tcs) ∧
+  subst_db skip ts (Function tfs t) =
+    Function (MAP (subst_db skip ts) tfs) (subst_db skip ts t) ∧
+  subst_db skip ts (Array t) = Array (subst_db skip ts t) ∧
+  subst_db skip ts (M t) = M (subst_db skip ts t)
+Termination
+  WF_REL_TAC `measure (type_size o SND o SND)` >> rw[fetch "-" "type_size_def"] >>
+  rename1 `MEM _ ts` >> Induct_on `ts` >> rw[fetch "-" "type_size_def"] >> gvs[]
+End
+
+Definition shift_db_def:
+  shift_db skip n (TypeVar v) = (
+    if skip ≤ v then TypeVar (v + n) else TypeVar v) ∧
+  shift_db skip n (PrimTy p) = PrimTy p ∧
+  shift_db skip n  Exception = Exception ∧
+  shift_db skip n (TypeCons tn tcs) = TypeCons tn (MAP (shift_db skip n) tcs) ∧
+  shift_db skip n (Tuple tcs) = Tuple  (MAP (shift_db skip n) tcs) ∧
+  shift_db skip n (Function tfs t) =
+    Function (MAP (shift_db skip n) tfs) (shift_db skip n t) ∧
+  shift_db skip n (Array t) = Array (shift_db skip n t) ∧
+  shift_db skip n (M t) = M (shift_db skip n t)
+Termination
+  WF_REL_TAC `measure (type_size o SND o SND)` >> rw[fetch "-" "type_size_def"] >>
+  rename1 `MEM _ ts` >> Induct_on `ts` >> rw[fetch "-" "type_size_def"] >> gvs[]
+End
+
+Overload tsubst = ``subst_db 0``;
+Overload tshift = ``shift_db 0``;
+Overload tshift_scheme = ``λn (vars,scheme). (vars, shift_db vars n scheme)``;
+Overload tshift_env = ``λn. MAP (λ(x,scheme). (x, tshift_scheme n scheme))``;
+
+
+(******************** Properties of types ********************)
+
+Definition freetyvars_ok_def:
+  freetyvars_ok n (TypeVar v) = (v < n) ∧
+  freetyvars_ok n (PrimTy p) = T ∧
+  freetyvars_ok n  Exception = T ∧
+  freetyvars_ok n (TypeCons c ts) = EVERY (freetyvars_ok n) ts ∧
+  freetyvars_ok n (Tuple ts) = EVERY (freetyvars_ok n) ts ∧
+  freetyvars_ok n (Function ts t) =
+    (EVERY (freetyvars_ok n) ts ∧ freetyvars_ok n t) ∧
+  freetyvars_ok n (Array t) = freetyvars_ok n t ∧
+  freetyvars_ok n (M t) = freetyvars_ok n t
+Termination
+  WF_REL_TAC `measure (type_size o SND)` >> rw[fetch "-" "type_size_def"] >>
+  rename1 `MEM _ ts` >> Induct_on `ts` >> rw[fetch "-" "type_size_def"] >> gvs[]
+End
+
+Overload freetyvars_ok_scheme =
+  ``λn (vars,scheme). freetyvars_ok (n + vars) scheme``;
+
+(* Does a type only contain defined constructors, and non-nullary functions? *)
+Definition type_wf_def:
+  type_wf (typedefs : typedefs) (TypeVar n) = T ∧
+  type_wf typedefs (PrimTy pty) = T ∧
+  type_wf typedefs  Exception = T ∧
+  type_wf typedefs (TypeCons id tyargs) = (
+    EVERY (type_wf typedefs) tyargs ∧
+    ∃arity constructors.
+      (* Type definition exists: *)
+        oEL id typedefs = SOME (arity, constructors) ∧
+      (* And has correct arity: *)
+        LENGTH tyargs = arity) ∧
+  type_wf typedefs (Tuple ts) =
+    EVERY (type_wf typedefs) ts ∧
+  type_wf typedefs (Function ts t) = (
+    type_wf typedefs t ∧
+    ts ≠ [] ∧ EVERY (type_wf typedefs) ts) ∧
+  type_wf typedefs (Array t) = type_wf typedefs t ∧
+  type_wf typedefs (M t) = type_wf typedefs t
+Termination
+  WF_REL_TAC `measure (type_size o SND)` >> rw[fetch "-" "type_size_def"] >>
+  rename1 `MEM _ ts` >> Induct_on `ts` >> rw[fetch "-" "type_size_def"] >> gvs[]
+End
+
+Definition type_ok_def:
+  type_ok typedefs db t ⇔
+    freetyvars_ok db t ∧
+    type_wf typedefs t
+End
+
+Overload type_scheme_ok =
+  ``λtdefs db (vars,scheme). type_ok tdefs (db + vars) scheme``
+
+(* Does a type specialise a type scheme in a given variable context/namespace? *)
+Definition specialises_def:
+  specialises tdefs db (vars, scheme) t =
+    ∃subs.
+      EVERY (type_ok tdefs db) subs ∧
+      LENGTH subs = vars ∧
+      tsubst subs scheme = t
+End
+
+(* Our namespace is an exception definition and some datatype definitions *)
+Definition namespace_ok_def:
+  namespace_ok (exndef : exndef, typedefs : typedefs) ⇔
+    (* No empty type definitions: *)
+      EVERY (λ(ar,td). td ≠ []) typedefs ∧
+    (* Unique, unreserved constructor names: *)
+      ALL_DISTINCT (SET_TO_LIST reserved_cns ++
+        MAP FST exndef ++ MAP FST (FLAT $ MAP SND typedefs)) ∧
+    (* Every constructor type is closed wrt type arity and uses only defined types: *)
+      EVERY (λ(ar,td).
+        EVERY (λ(cn,argtys). EVERY (type_ok typedefs ar) argtys) td) typedefs ∧
+    (* Every exception constructor type is closed and uses only defined types: *)
+      EVERY (λ(cn,tys). EVERY (type_ok typedefs 0) tys) exndef
+End
+
+
+(******************** Typing judgements ********************)
 
 (* Handle Locs separately *)
 Inductive type_lit:
@@ -76,197 +229,7 @@ Inductive type_atom_op:
   (type_atom_op (Message s) [String] Message)
 End
 
-Theorem eval_op_type_safe:
-  (type_atom_op op ts t ∧ t ≠ Bool ∧
-   LIST_REL type_lit ls ts ⇒
-  ∃res.
-    eval_op op ls = SOME (INL res) ∧
-    type_lit res t) ∧
-  (type_atom_op op ts Bool ∧
-   LIST_REL type_lit ls ts ⇒
-  ∃res.
-    eval_op op ls = SOME (INR res))
-Proof
-  rw[type_atom_op_cases, type_lit_cases] >> gvs[type_lit_cases, PULL_EXISTS]
-  >- (
-    ntac 2 $ last_x_assum mp_tac >> map_every qid_spec_tac [`ts`,`ls`] >>
-    Induct_on `LIST_REL` >> rw[] >> gvs[type_lit_cases, concat_def]
-    )
-  >- (
-    ntac 2 $ last_x_assum mp_tac >> map_every qid_spec_tac [`ts`,`ls`] >>
-    Induct_on `LIST_REL` >> rw[] >> gvs[type_lit_cases, implode_def]
-    )
-  >- (IF_CASES_TAC >> gvs[])
-QED
-
-Definition freetyvars_ok_def:
-  freetyvars_ok n (TypeVar v) = (v < n) ∧
-  freetyvars_ok n (PrimTy p) = T ∧
-  freetyvars_ok n  Exception = T ∧
-  freetyvars_ok n (TypeCons c ts) = EVERY (freetyvars_ok n) ts ∧
-  freetyvars_ok n (Tuple ts) = EVERY (freetyvars_ok n) ts ∧
-  freetyvars_ok n (Function ts t) =
-    (EVERY (freetyvars_ok n) ts ∧ freetyvars_ok n t) ∧
-  freetyvars_ok n (Array t) = freetyvars_ok n t ∧
-  freetyvars_ok n (M t) = freetyvars_ok n t
-Termination
-  WF_REL_TAC `measure (type_size o SND)` >> rw[fetch "-" "type_size_def"] >>
-  rename1 `MEM _ ts` >> Induct_on `ts` >> rw[fetch "-" "type_size_def"] >> gvs[]
-End
-
-Definition subst_db_def:
-  subst_db skip ts (TypeVar v) = (
-    if skip ≤ v ∧ v < skip + LENGTH ts then
-      EL (v - skip) ts
-    else if skip ≤ v then
-      TypeVar (v - LENGTH ts)
-    else TypeVar v) ∧
-  subst_db skip ts (PrimTy p) = PrimTy p ∧
-  subst_db skip ts  Exception = Exception ∧
-  subst_db skip ts (TypeCons n tcs) = TypeCons n (MAP (subst_db skip ts) tcs) ∧
-  subst_db skip ts (Tuple tcs) = Tuple  (MAP (subst_db skip ts) tcs) ∧
-  subst_db skip ts (Function tfs t) =
-    Function (MAP (subst_db skip ts) tfs) (subst_db skip ts t) ∧
-  subst_db skip ts (Array t) = Array (subst_db skip ts t) ∧
-  subst_db skip ts (M t) = M (subst_db skip ts t)
-Termination
-  WF_REL_TAC `measure (type_size o SND o SND)` >> rw[fetch "-" "type_size_def"] >>
-  rename1 `MEM _ ts` >> Induct_on `ts` >> rw[fetch "-" "type_size_def"] >> gvs[]
-End
-
-Definition shift_db_def:
-  shift_db skip n (TypeVar v) = (
-    if skip ≤ v then TypeVar (v + n) else TypeVar v) ∧
-  shift_db skip n (PrimTy p) = PrimTy p ∧
-  shift_db skip n  Exception = Exception ∧
-  shift_db skip n (TypeCons tn tcs) = TypeCons tn (MAP (shift_db skip n) tcs) ∧
-  shift_db skip n (Tuple tcs) = Tuple  (MAP (shift_db skip n) tcs) ∧
-  shift_db skip n (Function tfs t) =
-    Function (MAP (shift_db skip n) tfs) (shift_db skip n t) ∧
-  shift_db skip n (Array t) = Array (shift_db skip n t) ∧
-  shift_db skip n (M t) = M (shift_db skip n t)
-Termination
-  WF_REL_TAC `measure (type_size o SND o SND)` >> rw[fetch "-" "type_size_def"] >>
-  rename1 `MEM _ ts` >> Induct_on `ts` >> rw[fetch "-" "type_size_def"] >> gvs[]
-End
-
-Theorem shift_db_0[simp]:
-  shift_db skip 0 t = t
-Proof
-  qsuff_tac `∀skip n t. n = 0 ⇒ shift_db skip n t = t` >- gvs[] >>
-  recInduct shift_db_ind >> rw[shift_db_def] >>
-  rw[LIST_EQ_REWRITE] >> gvs[MEM_EL, PULL_EXISTS, EL_MAP]
-QED
-
-Type type_scheme[pp] = ``:num # type``;
-Overload freetyvars_ok_scheme =
-  ``λn (vars,scheme). freetyvars_ok (n + vars) scheme``;
-Overload tsubst = ``subst_db 0``;
-Overload tshift = ``shift_db 0``;
-Overload tshift_scheme = ``λn (vars,scheme). (vars, shift_db vars n scheme)``;
-Overload tshift_env = ``λn. MAP (λ(x,scheme). (x, tshift_scheme n scheme))``;
-
-Type typedef[pp] = ``:num # ((string # type list) list)``;
-Type typedefs[pp] = ``:typedef list``;
-Type exndef[pp] = ``:(string # type list) list``;
-(*
-  A type definition is an arity and a collection of constructor definitions.
-  Each constructor definition is a name and a type scheme for its arguments
-  (closed wrt the type definition arity).
-
-  Like CakeML, use numbers to refer to types - known typedefs represented as
-    : typedef list
-  We could instead have:
-    : (string # typedef) list     or     : string |-> typedef     etc.
-  Unlike CakeML, we group constructors by their type (i.e. group siblings).
-
-  E.g. the type definitions for Maybe and List might look like:
-  [
-    (1, [ ("Nothing", []) ; ("Just", [Var 0]) ]);
-    (1, [ ("Nil", []) ; ("Cons", [Var 0; TypeCons 1 [Var 0]]) ])
-  ]
-
-  The exception definition is a list of constructors associated to (closed)
-  argument types.
-*)
-
-(* Does a type only contain defined constructors? *)
-Definition type_wf_def:
-  type_wf (typedefs : typedefs) (TypeVar n) = T ∧
-  type_wf typedefs (PrimTy pty) = T ∧
-  type_wf typedefs  Exception = T ∧
-  type_wf typedefs (TypeCons id tyargs) = (
-    EVERY (type_wf typedefs) tyargs ∧
-    ∃arity constructors.
-      (* Type definition exists: *)
-        oEL id typedefs = SOME (arity, constructors) ∧
-      (* And has correct arity: *)
-        LENGTH tyargs = arity) ∧
-  type_wf typedefs (Tuple ts) =
-    EVERY (type_wf typedefs) ts ∧
-  type_wf typedefs (Function ts t) = (
-    type_wf typedefs t ∧
-    ts ≠ [] ∧ EVERY (type_wf typedefs) ts) ∧
-  type_wf typedefs (Array t) = type_wf typedefs t ∧
-  type_wf typedefs (M t) = type_wf typedefs t
-Termination
-  WF_REL_TAC `measure (type_size o SND)` >> rw[fetch "-" "type_size_def"] >>
-  rename1 `MEM _ ts` >> Induct_on `ts` >> rw[fetch "-" "type_size_def"] >> gvs[]
-End
-
-Definition type_ok_def:
-  type_ok typedefs db t ⇔
-    freetyvars_ok db t ∧
-    type_wf typedefs t
-End
-
-Theorem type_ok:
-  (∀tds v n. type_ok tds n (TypeVar v) ⇔ v < n) ∧
-  (∀tds p n. type_ok tds n (PrimTy p) ⇔ T) ∧
-  (∀tds n. type_ok tds n Exception ⇔ T) ∧
-  (∀tds ts n c.
-    type_ok tds n (TypeCons c ts) ⇔
-    EVERY (λa. type_ok tds n a) ts ∧
-    ∃ctors. oEL c tds = SOME (LENGTH ts, ctors)) ∧
-  (∀tds ts n. type_ok tds n (Tuple ts) ⇔ EVERY (λa. type_ok tds n a) ts) ∧
-  (∀tds ts t n.
-   type_ok tds n (Function ts t) ⇔
-   EVERY (λa. type_ok tds n a) ts ∧ ts ≠ [] ∧ type_ok tds n t) ∧
-  (∀tds t n. type_ok tds n (Array t) ⇔ type_ok tds n t) ∧
-  (∀tds t n. type_ok tds n (M t) ⇔ type_ok tds n t)
-Proof
-  rw[type_ok_def, type_wf_def, freetyvars_ok_def] >>
-  gvs[EVERY_CONJ] >> eq_tac >> gvs[]
-QED
-
-Overload type_scheme_ok =
-  ``λtdefs db (vars,scheme). type_ok tdefs (db + vars) scheme``
-
-(* Does a type specialise a type scheme in a given variable context/namespace? *)
-Definition specialises_def:
-  specialises tdefs db (vars, scheme) t =
-    ∃subs.
-      EVERY (type_ok tdefs db) subs ∧
-      LENGTH subs = vars ∧
-      tsubst subs scheme = t
-End
-
-
-(* Our namespace is an exception definition and some datatype definitions *)
-Definition namespace_ok_def:
-  namespace_ok (exndef : exndef, typedefs : typedefs) ⇔
-    (* No empty type definitions: *)
-      EVERY (λ(ar,td). td ≠ []) typedefs ∧
-    (* Unique, unreserved constructor names: *)
-      ALL_DISTINCT (data_reserved_cns ++
-        MAP FST exndef ++ MAP FST (FLAT $ MAP SND typedefs)) ∧
-    (* Every constructor type is closed wrt type arity and uses only defined types: *)
-      EVERY (λ(ar,td).
-        EVERY (λ(cn,argtys). EVERY (type_ok typedefs ar) argtys) td) typedefs ∧
-    (* Every exception constructor type is closed and uses only defined types: *)
-      EVERY (λ(cn,tys). EVERY (type_ok typedefs 0) tys) exndef
-End
-
+(* Typing judgments for type constructors *)
 Definition type_cons_def:
   type_cons (typedefs : typedefs) (cname,carg_tys) (tyid,tyargs) ⇔
     ∃arity constructors schemes.
@@ -279,6 +242,7 @@ Definition type_cons_def:
         LIST_REL (λs t. tsubst tyargs s = t) schemes carg_tys
 End
 
+(* Typing judgments for exceptions *)
 Definition type_exception_def:
   type_exception (exndef : exndef) (cname, carg_tys) ⇔
       ALOOKUP exndef cname = SOME carg_tys
@@ -289,7 +253,6 @@ Definition get_PrimTys_def:
   get_PrimTys (PrimTy pty :: rest) = OPTION_MAP (CONS pty) (get_PrimTys rest) ∧
   get_PrimTys _ = NONE
 End
-
 
 (*
   The main typing relation.
@@ -362,6 +325,9 @@ Inductive type_cexp:
 
 [~False:]
   (type_cexp ns db st env (Prim c (Cons "False") []) (PrimTy Bool)) ∧
+
+[~Subscript:]
+  (type_cexp ns db st env (Prim c (Cons "Subscript") []) Exception) ∧
 
 [~Cons:]
   (LIST_REL (type_cexp (exndef,typedefs) db st env) es carg_ts ∧
@@ -442,175 +408,6 @@ Inductive type_cexp:
       type_cexp (exndef,typedefs) db st env (Case c e v css) t)
 End
 
-Theorem freetyvars_ok_mono:
-  ∀n t m.
-    freetyvars_ok n t ∧
-    n ≤ m
-  ⇒ freetyvars_ok m t
-Proof
-  recInduct freetyvars_ok_ind >> rw[freetyvars_ok_def] >> gvs[EVERY_MEM]
-QED
-
-Theorem freetyvars_ok_subst_db:
-  ∀skip ts t n.
-    freetyvars_ok (n + LENGTH ts) t ∧
-    EVERY (freetyvars_ok n) ts ∧
-    skip ≤ n
-  ⇒ freetyvars_ok n (subst_db skip ts t)
-Proof
-  recInduct subst_db_ind >>
-  rw[subst_db_def, freetyvars_ok_def] >>
-  gvs[EVERY_MEM, MEM_MAP, PULL_EXISTS] >>
-  gvs[MEM_EL, PULL_EXISTS]
-QED
-
-Theorem freetyvars_ok_tsubst:
-  ∀ts t n.
-    freetyvars_ok (n + LENGTH ts) t ∧
-    EVERY (freetyvars_ok n) ts
-  ⇒ freetyvars_ok n (tsubst ts t)
-Proof
-  rw[] >> irule freetyvars_ok_subst_db >> simp[]
-QED
-
-Theorem freetyvars_ok_shift_db:
-  ∀skip shift t n.
-    freetyvars_ok n t
-  ⇒ freetyvars_ok (n + shift) (shift_db skip shift t)
-Proof
-  recInduct shift_db_ind >>
-  rw[shift_db_def, freetyvars_ok_def] >>
-  gvs[EVERY_MEM, MEM_MAP, PULL_EXISTS]
-QED
-
-Theorem type_cexp_freetyvars_ok:
-  ∀ ns db st env e t.
-    EVERY (freetyvars_ok db) st ∧
-    EVERY (λ(v,scheme). freetyvars_ok_scheme db scheme) env ∧
-    namespace_ok ns ∧
-    type_cexp ns db st env e t
-  ⇒ freetyvars_ok db t
-Proof
-  Induct_on `type_cexp` >> rpt conj_tac >>
-  rw[type_ok_def, freetyvars_ok_def] >>
-  gvs[LIST_REL_EL_EQN, IMP_CONJ_THM, FORALL_AND_THM]
-  >- (
-    PairCases_on `s` >> gvs[specialises_def] >>
-    imp_res_tac ALOOKUP_MEM >> gvs[EVERY_MEM, type_ok_def] >>
-    first_x_assum drule >> strip_tac >> gvs[] >>
-    irule freetyvars_ok_tsubst >> simp[EVERY_MEM]
-    )
-  >- gvs[EVERY_EL]
-  >- gvs[EVERY_EL, type_ok_def]
-  >- gvs[oEL_THM, EVERY_EL]
-  >- gvs[EVERY_EL, type_ok_def]
-  >- (
-    first_x_assum irule >>
-    gvs[EVERY_MEM, MEM_ZIP, PULL_EXISTS, EL_MAP, MEM_EL, type_ok_def]
-    )
-  >- (
-    ntac 2 $ first_x_assum irule >> gvs[EVERY_MEM, FORALL_PROD] >>
-    rw[] >> gvs[MEM_MAP, EXISTS_PROD] >>
-    first_x_assum drule >> rw[]
-    >- (
-      drule freetyvars_ok_shift_db >> rename1 `MEM (a,b,c) _` >>
-      disch_then $ qspecl_then [`b`,`new`] assume_tac >> gvs[]
-      )
-    >- (
-      drule freetyvars_ok_mono >> disch_then irule >> simp[]
-      )
-    )
-  >- (
-    first_x_assum irule >>
-    rw[EVERY_EL, EL_ZIP, EL_MAP] >> pairarg_tac >> gvs[EVERY_EL] >>
-    last_x_assum kall_tac >> last_x_assum drule >> simp[]
-    )
-  >- (
-    gvs[EVERY_MEM, oEL_THM, namespace_ok_def, type_ok_def] >>
-    Cases_on `css` >> gvs[] >- gvs[MEM_EL, FORALL_PROD] >>
-    last_x_assum $ qspec_then `h` assume_tac >> gvs[] >>
-    pairarg_tac >> gvs[] >>
-    qpat_x_assum `_ ⇒ freetyvars_ok db t` irule >>
-    simp[MEM_ZIP, EL_MAP, PULL_EXISTS] >>
-    gvs[MEM_EL, PULL_EXISTS]
-    )
-QED
-
-Theorem type_wf_subst_db:
-  ∀skip ts t tdefs.
-    type_wf tdefs t ∧
-    EVERY (type_wf tdefs) ts
-  ⇒ type_wf tdefs (subst_db skip ts t)
-Proof
-  recInduct subst_db_ind >> rw[subst_db_def, type_wf_def] >>
-  gvs[EVERY_MAP, EVERY_MEM] >> gvs[MEM_EL, PULL_EXISTS]
-QED
-
-Theorem type_wf_shift_db:
-  ∀skip shift t tdefs.
-    type_wf tdefs t
-  ⇒ type_wf tdefs (shift_db skip shift t)
-Proof
-  recInduct shift_db_ind >> rw[shift_db_def, type_wf_def] >>
-  gvs[EVERY_MAP, EVERY_MEM]
-QED
-
-Theorem type_cexp_type_ok:
-  ∀ ns db st env e t.
-    EVERY (type_ok (SND ns) db) st ∧
-    EVERY (λ(v,scheme). type_scheme_ok (SND ns) db scheme) env ∧
-    namespace_ok ns ∧
-    type_cexp ns db st env e t
-  ⇒ type_ok (SND ns) db t
-Proof
-  Induct_on `type_cexp` >> rpt conj_tac >> rw[type_ok] >>
-  gvs[LIST_REL_EL_EQN, IMP_CONJ_THM, FORALL_AND_THM]
-  >- (
-    PairCases_on `s` >> gvs[specialises_def] >>
-    imp_res_tac ALOOKUP_MEM >> gvs[EVERY_MEM, type_ok_def] >>
-    first_x_assum drule >> strip_tac >> gvs[] >>
-    irule_at Any freetyvars_ok_tsubst >> simp[EVERY_MEM] >>
-    irule_at Any type_wf_subst_db >> simp[EVERY_MEM]
-    )
-  >- gvs[EVERY_EL]
-  >- gvs[EVERY_EL, type_ok_def]
-  >- gvs[type_cons_def]
-  >- gvs[oEL_THM, EVERY_EL]
-  >- gvs[EVERY_EL, type_ok_def]
-  >- (
-    first_x_assum irule >>
-    gvs[EVERY_MEM, MEM_ZIP, PULL_EXISTS, EL_MAP, MEM_EL, type_ok_def]
-    )
-  >- (
-    ntac 2 $ first_x_assum irule >> gvs[EVERY_MEM, FORALL_PROD] >>
-    rw[] >> gvs[MEM_MAP, EXISTS_PROD] >>
-    first_x_assum drule >> rw[]
-    >- (
-      gvs[type_ok_def] >>
-      drule freetyvars_ok_shift_db >> rename1 `MEM (a,b,c) _` >>
-      disch_then $ qspecl_then [`b`,`new`] assume_tac >> gvs[] >>
-      irule type_wf_shift_db >> simp[]
-      )
-    >- (
-      gvs[type_ok_def] >>
-      drule freetyvars_ok_mono >> disch_then irule >> simp[]
-      )
-    )
-  >- (
-    first_x_assum irule >>
-    rw[EVERY_EL, EL_ZIP, EL_MAP] >> pairarg_tac >> gvs[EVERY_EL] >>
-    last_x_assum kall_tac >> last_x_assum drule >> simp[]
-    )
-  >- (
-    gvs[EVERY_MEM, oEL_THM, namespace_ok_def] >>
-    Cases_on `css` >> gvs[] >- gvs[MEM_EL, FORALL_PROD] >>
-    last_x_assum $ qspec_then `h` assume_tac >> gvs[] >>
-    pairarg_tac >> gvs[] >>
-    qpat_x_assum `_ ⇒ type_ok typedefs db t` irule >>
-    simp[MEM_ZIP, EL_MAP, PULL_EXISTS] >>
-    gvs[MEM_EL, PULL_EXISTS]
-    )
-QED
 
 (********************)
 
