typing/pure_typingProofScript.sml
@@ -1,0 +1,34 @@
+open HolKernel Parse boolLib bossLib BasicProvers;
+open pairTheory arithmeticTheory integerTheory stringTheory optionTheory
+     listTheory alistTheory;
+open pure_cexpTheory pure_configTheory pure_typingTheory pure_typingPropsTheory
+
+val _ = new_theory "pure_typingProof";
+
+Theorem eval_op_type_safe:
+  (type_atom_op op ts t ∧ t ≠ Bool ∧
+   LIST_REL type_lit ls ts ⇒
+  ∃res.
+    eval_op op ls = SOME (INL res) ∧
+    type_lit res t) ∧
+  (type_atom_op op ts Bool ∧
+   LIST_REL type_lit ls ts ⇒
+  ∃res.
+    eval_op op ls = SOME (INR res))
+Proof
+  rw[type_atom_op_cases, type_lit_cases] >> gvs[type_lit_cases, PULL_EXISTS]
+  >- (
+    ntac 2 $ last_x_assum mp_tac >> map_every qid_spec_tac [`ts`,`ls`] >>
+    Induct_on `LIST_REL` >> rw[] >> gvs[type_lit_cases, concat_def]
+    )
+  >- (
+    ntac 2 $ last_x_assum mp_tac >> map_every qid_spec_tac [`ts`,`ls`] >>
+    Induct_on `LIST_REL` >> rw[] >> gvs[type_lit_cases, implode_def]
+    )
+  >- (IF_CASES_TAC >> gvs[])
+QED
+
+
+(********************)
+
+val _ = export_theory();
