typing/pure_typingPropsScript.sml
@@ -1,0 +1,218 @@
+open HolKernel Parse boolLib bossLib BasicProvers;
+open pairTheory arithmeticTheory integerTheory stringTheory optionTheory
+     listTheory alistTheory;
+open pure_cexpTheory pure_configTheory pure_typingTheory
+
+val _ = new_theory "pure_typingProps";
+
+
+(******************** Substitutions and shifts ********************)
+
+Theorem shift_db_0[simp]:
+  shift_db skip 0 t = t
+Proof
+  qsuff_tac `∀skip n t. n = 0 ⇒ shift_db skip n t = t` >- gvs[] >>
+  recInduct shift_db_ind >> rw[shift_db_def] >>
+  rw[LIST_EQ_REWRITE] >> gvs[MEM_EL, PULL_EXISTS, EL_MAP]
+QED
+
+
+(******************** Properties of types ********************)
+
+Theorem freetyvars_ok_mono:
+  ∀n t m.
+    freetyvars_ok n t ∧
+    n ≤ m
+  ⇒ freetyvars_ok m t
+Proof
+  recInduct freetyvars_ok_ind >> rw[freetyvars_ok_def] >> gvs[EVERY_MEM]
+QED
+
+Theorem freetyvars_ok_subst_db:
+  ∀skip ts t n.
+    freetyvars_ok (n + LENGTH ts) t ∧
+    EVERY (freetyvars_ok n) ts ∧
+    skip ≤ n
+  ⇒ freetyvars_ok n (subst_db skip ts t)
+Proof
+  recInduct subst_db_ind >>
+  rw[subst_db_def, freetyvars_ok_def] >>
+  gvs[EVERY_MEM, MEM_MAP, PULL_EXISTS] >>
+  gvs[MEM_EL, PULL_EXISTS]
+QED
+
+Theorem freetyvars_ok_tsubst:
+  ∀ts t n.
+    freetyvars_ok (n + LENGTH ts) t ∧
+    EVERY (freetyvars_ok n) ts
+  ⇒ freetyvars_ok n (tsubst ts t)
+Proof
+  rw[] >> irule freetyvars_ok_subst_db >> simp[]
+QED
+
+Theorem freetyvars_ok_shift_db:
+  ∀skip shift t n.
+    freetyvars_ok n t
+  ⇒ freetyvars_ok (n + shift) (shift_db skip shift t)
+Proof
+  recInduct shift_db_ind >>
+  rw[shift_db_def, freetyvars_ok_def] >>
+  gvs[EVERY_MEM, MEM_MAP, PULL_EXISTS]
+QED
+
+Theorem type_wf_subst_db:
+  ∀skip ts t tdefs.
+    type_wf tdefs t ∧
+    EVERY (type_wf tdefs) ts
+  ⇒ type_wf tdefs (subst_db skip ts t)
+Proof
+  recInduct subst_db_ind >> rw[subst_db_def, type_wf_def] >>
+  gvs[EVERY_MAP, EVERY_MEM] >> gvs[MEM_EL, PULL_EXISTS]
+QED
+
+Theorem type_wf_shift_db:
+  ∀skip shift t tdefs.
+    type_wf tdefs t
+  ⇒ type_wf tdefs (shift_db skip shift t)
+Proof
+  recInduct shift_db_ind >> rw[shift_db_def, type_wf_def] >>
+  gvs[EVERY_MAP, EVERY_MEM]
+QED
+
+Theorem type_ok:
+  (∀tds v n. type_ok tds n (TypeVar v) ⇔ v < n) ∧
+  (∀tds p n. type_ok tds n (PrimTy p) ⇔ T) ∧
+  (∀tds n. type_ok tds n Exception ⇔ T) ∧
+  (∀tds ts n c.
+    type_ok tds n (TypeCons c ts) ⇔
+    EVERY (λa. type_ok tds n a) ts ∧
+    ∃ctors. oEL c tds = SOME (LENGTH ts, ctors)) ∧
+  (∀tds ts n. type_ok tds n (Tuple ts) ⇔ EVERY (λa. type_ok tds n a) ts) ∧
+  (∀tds ts t n.
+   type_ok tds n (Function ts t) ⇔
+   EVERY (λa. type_ok tds n a) ts ∧ ts ≠ [] ∧ type_ok tds n t) ∧
+  (∀tds t n. type_ok tds n (Array t) ⇔ type_ok tds n t) ∧
+  (∀tds t n. type_ok tds n (M t) ⇔ type_ok tds n t)
+Proof
+  rw[type_ok_def, type_wf_def, freetyvars_ok_def] >>
+  gvs[EVERY_CONJ] >> eq_tac >> gvs[]
+QED
+
+
+(******************** Typing judgements ********************)
+
+Theorem type_cexp_freetyvars_ok:
+  ∀ ns db st env e t.
+    EVERY (freetyvars_ok db) st ∧
+    EVERY (λ(v,scheme). freetyvars_ok_scheme db scheme) env ∧
+    namespace_ok ns ∧
+    type_cexp ns db st env e t
+  ⇒ freetyvars_ok db t
+Proof
+  Induct_on `type_cexp` >> rpt conj_tac >>
+  rw[type_ok_def, freetyvars_ok_def] >>
+  gvs[LIST_REL_EL_EQN, IMP_CONJ_THM, FORALL_AND_THM]
+  >- (
+    PairCases_on `s` >> gvs[specialises_def] >>
+    imp_res_tac ALOOKUP_MEM >> gvs[EVERY_MEM, type_ok_def] >>
+    first_x_assum drule >> strip_tac >> gvs[] >>
+    irule freetyvars_ok_tsubst >> simp[EVERY_MEM]
+    )
+  >- gvs[EVERY_EL]
+  >- gvs[EVERY_EL, type_ok_def]
+  >- gvs[oEL_THM, EVERY_EL]
+  >- gvs[EVERY_EL, type_ok_def]
+  >- (
+    first_x_assum irule >>
+    gvs[EVERY_MEM, MEM_ZIP, PULL_EXISTS, EL_MAP, MEM_EL, type_ok_def]
+    )
+  >- (
+    ntac 2 $ first_x_assum irule >> gvs[EVERY_MEM, FORALL_PROD] >>
+    rw[] >> gvs[MEM_MAP, EXISTS_PROD] >>
+    first_x_assum drule >> rw[]
+    >- (
+      drule freetyvars_ok_shift_db >> rename1 `MEM (a,b,c) _` >>
+      disch_then $ qspecl_then [`b`,`new`] assume_tac >> gvs[]
+      )
+    >- (
+      drule freetyvars_ok_mono >> disch_then irule >> simp[]
+      )
+    )
+  >- (
+    first_x_assum irule >>
+    rw[EVERY_EL, EL_ZIP, EL_MAP] >> pairarg_tac >> gvs[EVERY_EL] >>
+    last_x_assum kall_tac >> last_x_assum drule >> simp[]
+    )
+  >- (
+    gvs[EVERY_MEM, oEL_THM, namespace_ok_def, type_ok_def] >>
+    Cases_on `css` >> gvs[] >- gvs[MEM_EL, FORALL_PROD] >>
+    last_x_assum $ qspec_then `h` assume_tac >> gvs[] >>
+    pairarg_tac >> gvs[] >>
+    qpat_x_assum `_ ⇒ freetyvars_ok db t` irule >>
+    simp[MEM_ZIP, EL_MAP, PULL_EXISTS] >>
+    gvs[MEM_EL, PULL_EXISTS]
+    )
+QED
+
+Theorem type_cexp_type_ok:
+  ∀ ns db st env e t.
+    EVERY (type_ok (SND ns) db) st ∧
+    EVERY (λ(v,scheme). type_scheme_ok (SND ns) db scheme) env ∧
+    namespace_ok ns ∧
+    type_cexp ns db st env e t
+  ⇒ type_ok (SND ns) db t
+Proof
+  Induct_on `type_cexp` >> rpt conj_tac >> rw[type_ok] >>
+  gvs[LIST_REL_EL_EQN, IMP_CONJ_THM, FORALL_AND_THM]
+  >- (
+    PairCases_on `s` >> gvs[specialises_def] >>
+    imp_res_tac ALOOKUP_MEM >> gvs[EVERY_MEM, type_ok_def] >>
+    first_x_assum drule >> strip_tac >> gvs[] >>
+    irule_at Any freetyvars_ok_tsubst >> simp[EVERY_MEM] >>
+    irule_at Any type_wf_subst_db >> simp[EVERY_MEM]
+    )
+  >- gvs[EVERY_EL]
+  >- gvs[EVERY_EL, type_ok_def]
+  >- gvs[type_cons_def]
+  >- gvs[oEL_THM, EVERY_EL]
+  >- gvs[EVERY_EL, type_ok_def]
+  >- (
+    first_x_assum irule >>
+    gvs[EVERY_MEM, MEM_ZIP, PULL_EXISTS, EL_MAP, MEM_EL, type_ok_def]
+    )
+  >- (
+    ntac 2 $ first_x_assum irule >> gvs[EVERY_MEM, FORALL_PROD] >>
+    rw[] >> gvs[MEM_MAP, EXISTS_PROD] >>
+    first_x_assum drule >> rw[]
+    >- (
+      gvs[type_ok_def] >>
+      drule freetyvars_ok_shift_db >> rename1 `MEM (a,b,c) _` >>
+      disch_then $ qspecl_then [`b`,`new`] assume_tac >> gvs[] >>
+      irule type_wf_shift_db >> simp[]
+      )
+    >- (
+      gvs[type_ok_def] >>
+      drule freetyvars_ok_mono >> disch_then irule >> simp[]
+      )
+    )
+  >- (
+    first_x_assum irule >>
+    rw[EVERY_EL, EL_ZIP, EL_MAP] >> pairarg_tac >> gvs[EVERY_EL] >>
+    last_x_assum kall_tac >> last_x_assum drule >> simp[]
+    )
+  >- (
+    gvs[EVERY_MEM, oEL_THM, namespace_ok_def] >>
+    Cases_on `css` >> gvs[] >- gvs[MEM_EL, FORALL_PROD] >>
+    last_x_assum $ qspec_then `h` assume_tac >> gvs[] >>
+    pairarg_tac >> gvs[] >>
+    qpat_x_assum `_ ⇒ type_ok typedefs db t` irule >>
+    simp[MEM_ZIP, EL_MAP, PULL_EXISTS] >>
+    gvs[MEM_EL, PULL_EXISTS]
+    )
+QED
+
+
+(********************)
+
+val _ = export_theory();
+
